Move shape-related computations into separate file

SessionTypes.v
@@ -1,4 +1,4 @@
-Require Import Env Msg Shape Var.
+Require Import Env Msg Var.
 
 Inductive Sty : Set :=
 | unit : Sty
@@ -9,21 +9,3 @@ Inductive Sty : Set :=
 | mu : Var -> Sty -> Sty
 | var : Var -> Sty
 .
-
-
-Definition shape (S : Sty) : Shape :=
-  match S with
-  | unit => unitS
-  | send _ _ => sendS
-  | recv _ _ => recvS
-  | ichoice _ _ => ichoiceS
-  | echoice _ _ => echoiceS
-  | mu _ _ => muS
-  | var _ => varS
-  end
-.
-
-
-Lemma shape_dec :
-  forall S sh, {shape S = sh} + {shape S <> sh}.
-Proof. decide equality. Qed.
