Shape.v
@@ -1,3 +1,5 @@
+Require Import SessionTypes.
+
 Inductive Shape : Set :=
 | unitS
 | sendS
@@ -7,3 +9,21 @@ Inductive Shape : Set :=
 | muS
 | varS
 .
+
+
+Definition shape (S : Sty) : Shape :=
+  match S with
+  | unit => unitS
+  | send _ _ => sendS
+  | recv _ _ => recvS
+  | ichoice _ _ => ichoiceS
+  | echoice _ _ => echoiceS
+  | mu _ _ => muS
+  | var _ => varS
+  end
+.
+
+
+Lemma shape_dec :
+  forall S sh, {shape S = sh} + {shape S <> sh}.
+Proof. decide equality. Qed.
